Define a state-based interface for reachability properties, prove it implies the general interface, and change ex to use it

coq/mixed_shallow/generic_ex.v
@@ -68,20 +68,23 @@ destruct s3. simpl in H1; rewrite H1 in H2;assumption.
 destruct (orb s1 s2);auto using clos_unstrict.
 Qed.
 
-Module ExPathSemantics <: ReachabilitySemantics.
+Module ExReachability <: StateBasedReachability.
 
-(* Definitions *)
+Definition cfg := cfg.
+Definition S := S.
+
 Definition index : Set := {gamma : cfg | terminates gamma S}.
 Definition ix_rel (i1 i2 : index) : Prop :=
   S (proj1_sig i1) (proj1_sig i2).
 
-Definition holds' strict env (phi phi' : formula cfg env) : cfg -> Prop :=
-  fun parent =>
-    forall rho gamma1,
-      clos S false parent gamma1 ->
-      phi rho gamma1 ->
-      exists gamma2, clos S strict gamma1 gamma2 /\ phi' rho gamma2.
-Definition holds strict env phi1 phi2 (i : index) := @holds' strict env phi1 phi2 (proj1_sig i).
+Definition state_reaches strict (i : index) gamma P :=
+  clos S false (proj1_sig i) gamma ->
+  exists gamma', clos S strict gamma gamma' /\ P gamma'.
+
+Definition holds strict env (phi phi' : formula cfg env) i :=
+  forall rho gamma,
+    phi rho gamma ->
+    state_reaches strict i gamma (phi' rho).
 
 (* Nontrivial proofs *)
 (** Circularity **)
@@ -91,9 +94,9 @@ Lemma ix_rel_ind : forall env (phi phi' : formula cfg env),
                    (forall i', ix_rel i i' -> holds true phi phi' i') ->
                    holds true phi phi' i)
        -> holds true phi phi' i0.
-intros env phi phi' i Hix_later.
+unfold holds, state_reaches; intros env phi phi' i Hix_later.
 destruct i as [a Hterm].
-unfold holds. simpl.
+simpl.
 apply (under_terminates Hterm).
 intros a0 Haa0 Hnext.
 
@@ -109,14 +112,9 @@ specialize (Hix_later i' Hreach).
 rewrite Hend.
 apply Hix_later.
 intros.
-apply Hnext.
-rewrite Hend.
-exact H.
+subst a0.
+eauto.
 Qed.
-
-Create HintDb holds_solve discriminated.
-Hint Transparent holds holds' : holds_solve.
-Hint Unfold holds' : holds_solve.
 
 Ltac clear_except_path :=
 repeat match goal with
@@ -157,97 +155,89 @@ Ltac holds_start := intros;
   repeat match goal with
   (* open unnecessary uses of holds/indices *)
   | [i : index |- _] => destruct i
-  | [H : holds _ _ _ (exist _ _ _) |- _] => unfold holds in H;simpl proj1_sig in H
-  | [|- holds _ _ _ (exist _ _ _)] => unfold holds;simpl proj1_sig;unfold holds';intros
   | [H : ix_rel (exist _ _ _) _ |- _] => unfold ix_rel in H; simpl proj1_sig in H
   | [H : ix_rel _ (exist _ _ _) |- _] => unfold ix_rel in H; simpl proj1_sig in H
-  (* Instantate a hypothesis quantified over ix_rel, as appears in strict trans *)
-  | [H : forall i', ix_rel (exist _ ?x ?t) i' -> holds _ ?phi _ i',
-       Hphi : ?phi _ ?x0 |- _ ] =>
-    let Hprog := fresh "Hprog" in
-    assert (clos S true x x0) as Hprog by clos_solve;
-    let x1 := fresh "x1" with Hstep := fresh "Hstep" with Hreach := fresh "Hreach" in
-    apply clos_true_step in Hprog; destruct Hprog as [x1 [Hstep Hreach]];
-    specialize (H (exist _ x1 (terminates_next t _ Hstep)) Hstep)
-  (* Use holds' hypotheses *)
-  | [H : holds' _ ?phi _ ?x, Hphi : ?phi _ ?gamma |- _]=>
-    let Hreach := fresh "Hreach" in
-    assert (clos S false x gamma) as Hreach by clos_solve;
-    specialize (H _ _ Hreach Hphi)
-  | [H : exists _, clos S _ _ _ /\ _ |- _] => destruct H as [? []]
+  | [H : state_reaches _ (exist _ _ _) _ _ |- _] =>
+    unfold state_reaches in H;simpl proj1_sig in H
+  | [|- state_reaches  _ (exist _ _ _) _ _] =>
+    unfold state_reaches;simpl proj1_sig;intros
+  (* Use hypotheses *)
+  | [H : (clos S ?f ?x ?y) -> _ |- _] =>
+    match goal with
+      | [H' : clos S f x y |- _] =>
+        specialize (H H')
+      | _ =>
+        let Hpath := fresh "Hpath" in
+        assert (clos S f x y) as Hpath by clos_solve;
+          specialize (H Hpath)
+    end
+  (* Open results *)
+  | [H : exists gamma : Top.cfg, _ |- _] =>
+    destruct H
+  | [H : _ /\ _ |- _] =>
+    destruct H
   end.
-Ltac holds_finish :=
-  solve[eauto with holds_solve
-       |intuition
-          (repeat match goal with
-             | [H : forall _ _, ?phi _ _ -> _, Hphi : ?phi _ _ |- _] =>
-               specialize (H _ _ Hphi)
-           end;firstorder with holds_solve)
-       ].
-Ltac holds_tac := holds_start;holds_finish.
 
-(** Transitivity **)
-Lemma holds_trans_strict : forall env phi phi' phi'' i,
-    @holds true env phi phi' i ->
-    (forall i' : index, ix_rel i i' -> holds false phi' phi'' i') ->
-   holds true phi phi'' i.
-holds_tac.
-Qed.
+Lemma reach_later : forall i i', ix_rel i i' ->
+    forall gamma P,
+      state_reaches true i gamma P ->
+      state_reaches true i' gamma P.
+  Proof.
+    holds_start; eauto with holds_solve.
+  Qed.
+  Lemma reach_unstrict : forall i gamma P,
+    state_reaches true i gamma P -> state_reaches false i gamma P.
+  Proof.
+    holds_start; eauto with holds_solve.
+  Qed.
 
-Lemma holds_trans : forall env phi phi' phi'' i,
-    @holds false env phi phi' i ->
-    holds false phi' phi'' i ->
-    holds false phi phi'' i.
-holds_tac.
-Qed.
+  Lemma reach_refl : forall i gamma (P : cfg -> Prop),
+                           P gamma -> state_reaches false i gamma P.
+  Proof.
+    holds_start; firstorder with holds_solve.
+  Qed.    
 
-Lemma holds_strict_later : forall env phi1 phi2 i,
-                             @holds true env phi1 phi2 i ->
-                             forall i', ix_rel i i' ->
-                                        holds true phi1 phi2 i'.
-holds_tac.
-Qed.
+  Lemma reach_step : forall i gamma (P : cfg -> Prop),
+    (exists gamma', S gamma gamma') ->
+    (forall gamma', S gamma gamma' -> P gamma') ->
+      state_reaches true i gamma P.
+  Proof.
+    holds_start; eauto with holds_solve.
+  Qed.
 
-Lemma holds_unstrict : forall env phi1 phi2 i,
-                         @holds true env phi1 phi2 i -> holds false phi1 phi2 i.
-holds_tac.
-Qed.
+  Lemma reach_impl : forall (P Q : cfg -> Prop),
+                           (forall c, P c -> Q c) ->
+                           forall strict i gamma,
+                             state_reaches strict i gamma P ->
+                             state_reaches strict i gamma Q.
+  Proof.
+    holds_start; eauto with holds_solve.
+  Qed.
 
-Lemma holds_step : forall env (phi phi' : formula cfg env),
-    (forall (e : env) (c : cfg),
-      phi e c ->
-      (exists c2 : cfg, S c c2) /\ (forall c2 : cfg, S c c2 -> phi' e c2)) ->
-    forall i, holds true phi phi' i.
-holds_tac.
-Qed.
+  Lemma reach_join : forall i gamma P,
+    state_reaches false i gamma
+     (fun gamma' => state_reaches false i gamma' P) ->
+    state_reaches false i gamma P.
+  Proof.
+    holds_start;eauto with holds_solve.
+  Qed.
 
-Lemma holds_refl : forall env phi i, @holds false env phi phi i.
-holds_tac.
-Qed.
+  Lemma reach_join_strict : forall i gamma P,
+    state_reaches true i gamma
+     (fun gamma' => forall i', ix_rel i i' -> state_reaches false i' gamma' P) ->
+    state_reaches true i gamma P.
+  Proof.
+    holds_start.
+    unfold ix_rel in H1; simpl proj1_sig in H1.
+    assert (clos S true x x0) by clos_solve;clear H0.
+    destruct (clos_true_step H2) as [x' [Hxx' Hx'x0]].
+    specialize (H1 (exist _ x' (terminates_next t _ Hxx')) Hxx' Hx'x0).
+    firstorder with holds_solve.
+  Qed.
+        
+End ExReachability.
 
-Lemma holds_case :
-    forall strict env (phi phi1 phi' : formula cfg env) i,
-      holds strict phi phi' i -> holds strict phi1 phi' i ->
-      holds strict (fun (e : env) (g : cfg) => phi e g \/ phi1 e g) phi' i.
-holds_tac.
-Qed.
-
-Lemma holds_mut_conseq :
-    forall strict env1 (phi1 phi2 : formula cfg env1)
-                  env2 (phi1' phi2' : formula cfg env2),
-     (forall gamma rho,
-        phi1 rho gamma ->
-        exists rho', phi1' rho' gamma /\
-                     forall gamma', phi2' rho' gamma' -> phi2 rho gamma') ->
-    forall i, holds strict phi1' phi2' i ->
-              holds strict phi1 phi2 i.
-holds_tac.
-Qed.
-
-Definition cfg := cfg.
-Definition S := S.
-End ExPathSemantics.
-
+Module ExPathSemantics := StateBasedSemantics ExReachability.
 Module ExPathSoundness := Soundness ExPathSemantics.
 
 Definition holds strict env (phi phi' : formula cfg env) :=
@@ -259,7 +249,7 @@ Lemma approx_holds env (phi phi' : formula cfg env) strict :
   holds strict phi phi'.
 intro H. unfold holds.
 intros.
-specialize (H (exist _ gamma H0) _ _ (clos_refl _ _) H1).
+specialize (H (exist _ gamma H0) _ _ H1 (clos_refl _ _)). 
 firstorder.
 Qed.
 
@@ -268,8 +258,8 @@ Lemma holds_approx env (phi phi' : formula cfg env) strict :
   (forall i, ExPathSemantics.holds strict phi phi' i).
 intros Hstrong i.
 destruct i as [gamma term].
-unfold ExPathSemantics.holds, ExPathSemantics.holds'.
-intros rho gamma1 Hreach Hphi.
+unfold ExPathSemantics.holds, ExReachability.holds.
+intros rho gamma1 Hphi Hreach.
 specialize (Hstrong _ gamma1 (terminates_fwd term Hreach) Hphi).
 firstorder.
 Qed.
